using the new version of prove_refinement

examples/heapster/linked_list_proofs.v
@@ -16,6 +16,7 @@ Import SAWCorePrelude.
 
 Lemma no_errors_is_elem : refinesFun is_elem (fun _ _ => noErrorsSpec).
 Proof.
+  unfold is_elem, is_elem__tuple_fun, noErrorsSpec.
   prove_refinement.
 Qed.
 
@@ -26,25 +27,31 @@ Proof.
   apply refinesM_letRecM0.
   apply refinesM_either_l; intros.
   - eapply refinesM_existsM_r. reflexivity.
-  - apply refinesM_sigT_rect_l; intros.
-    apply refinesM_if_l; intros.
+  - apply refinesM_if_l; intros.
     + eapply refinesM_existsM_r. reflexivity.
     + rewrite existsM_bindM.
       apply refinesM_existsM_l; intros. rewrite returnM_bindM.
-      apply refinesM_sigT_rect_l; intros.
       eapply refinesM_existsM_r. reflexivity.
 Qed.
 
 
+(*
 Fixpoint is_elem_spec (x:bitvector 64) (l:W64List) : CompM {_:bitvector 64 & unit} :=
   match l with
   | W64Nil => returnM (existT _ (bvNat 64 0) tt)
   | W64Cons y l' =>
-    if bvEq 64 x y then returnM (existT _ (bvNat 64 1) tt) else
+    if bvEq 64 y x then returnM (existT _ (bvNat 64 1) tt) else
       is_elem_spec x l'
   end.
+*)
 
-(* Arguments is_elem_spec /. *)
+Definition is_elem_spec (x:bitvector 64) : W64List -> CompM {_:bitvector 64 & unit} :=
+  W64List_rect (fun _ => CompM {_:bitvector 64 & unit})
+               (returnM (existT _ (bvNat 64 0) tt))
+               (fun y l' rec =>
+                  if bvEq 64 y x then returnM (existT _ (bvNat 64 1) tt) else rec).
+
+Arguments is_elem_spec /.
 
 Lemma bvEq_sym n x y : bvEq n x y = bvEq n y x.
   admit.
@@ -56,17 +63,11 @@ Lemma bvEq_eqb n x y : bvEq n (bvNat n x) (bvNat n y) = eqb x y.
   admit.
 Admitted.
 
+Definition bindM_returnM_CompM A (m:CompM A) : m >>= (fun x => returnM x) ~= m :=
+  bindM_returnM (M:=CompM) A m.
+
 Lemma is_elem_correct : refinesFun is_elem is_elem_spec.
 Proof.
-  prove_refinesFun.
-  induction a0; unfold is_elem_spec; simpl; prove_refinement.
-  - rewrite bvEq_sym in H. rewrite H in * |- *.
-    rewrite bvEq_eqb in H0. discriminate H0.
-  - rewrite bvEq_sym in H. rewrite H in * |- *.
-    rewrite bvEq_eqb in H0. discriminate H0.
-  - transitivity (is_elem_spec a a0 >>= returnM);
-      [ | rewrite bindM_returnM; reflexivity ].
-    apply Proper_refinesM_bindM; [ reflexivity | ].
-    intros sig1 sig2 esig; rewrite esig.
-    destruct sig2; simpl. destruct u. reflexivity.
+  unfold is_elem, is_elem__tuple_fun, is_elem_spec.
+  prove_refinement.
 Qed.
